Fixed linter problems

src/computability/encode_alphabet.lean
@@ -21,30 +21,35 @@ This file contains the definition of a (finite) encoding, a map from a type to s
 - `fin_encoding_bool_Γ₀₁`  : an encoding of bool.
 -/
 
-namespace encoding
+/-- An encoding of a type in a certain alphabet, together with a decoding. -/
 structure encoding (α : Type) :=
 (Γ : Type)
 (encode : α → list Γ)
 (decode : list Γ → option α)
-(encodek : ∀ x, decode(encode x) = some x )
+(encodek : ∀ x, decode(encode x) = some x)
 
+/-- An encoding plus a guarantue of finiteness of the alphabet. -/
 structure fin_encoding (α : Type) extends encoding α :=
 (Γ_fin : fintype Γ)
 
+/-- An alphabet consisting of bit0 and bit1 -/
 @[derive [inhabited,decidable_eq,fintype]]
 inductive Γ₀₁
 | bit0 | bit1
 
+/-- A standard Turing machine alphabet, consisting of blank,bit0,bit1,bra,ket,comma. -/
 @[derive [decidable_eq,fintype]]
 inductive Γ'
 | blank | bit0 | bit1 | bra | ket | comma
 
 instance inhabited_Γ' : inhabited Γ' := ⟨Γ'.blank⟩
 
+/-- The natural inclusion of Γ₀₁ in Γ'. -/
 def inclusion_Γ₀₁_Γ' : Γ₀₁ → Γ'
 | Γ₀₁.bit0 := Γ'.bit0
 | Γ₀₁.bit1 := Γ'.bit1
 
+/-- An arbitrary section of the natural inclusion of Γ₀₁ in Γ'. -/
 def section_Γ'_Γ₀₁ : Γ' → Γ₀₁
 | Γ'.bit0 := Γ₀₁.bit0
 | Γ'.bit1 := Γ₀₁.bit1
@@ -56,36 +61,38 @@ lemma left_inverse_section_inclusion : function.left_inverse section_Γ'_Γ₀�
 lemma inclusion_Γ₀₁_Γ'_injective : function.injective inclusion_Γ₀₁_Γ' :=
 function.has_left_inverse.injective (Exists.intro section_Γ'_Γ₀₁ left_inverse_section_inclusion)
 
+/-- An encoding function of the positive binary numbers in Γ₀₁. -/
 def encode_pos_num : pos_num → list Γ₀₁
 | pos_num.one := [Γ₀₁.bit1]
 | (pos_num.bit0 n) := Γ₀₁.bit0 :: encode_pos_num n
 | (pos_num.bit1 n) := Γ₀₁.bit1 :: encode_pos_num n
 
+/-- An encoding function of the binary numbers in Γ₀₁. -/
 def encode_num : num → list Γ₀₁
 | num.zero := []
 | (num.pos n) := encode_pos_num n
 
+/-- An encoding function of ℕ in Γ₀₁. -/
 def encode_nat (n : ℕ) : list Γ₀₁ := encode_num n
 
+/-- A decoding function from `list Γ₀₁` to the positive binary numbers. -/
 def decode_pos_num : list Γ₀₁ → pos_num
--- | [Γ₀₁.bit1] := pos_num.one
--- | (Γ₀₁.bit0 :: l) := (pos_num.bit0 (decode_pos_num l))
--- | (Γ₀₁.bit1 :: l) := (pos_num.bit1 (decode_pos_num l))
--- | _ := pos_num.one
 | (Γ₀₁.bit0 :: l) := (pos_num.bit0 (decode_pos_num l))
 | (Γ₀₁.bit1 :: l) := ite (l = []) pos_num.one (pos_num.bit1 (decode_pos_num l))
 | _ := pos_num.one
 
+/-- A decoding function from `list Γ₀₁` to the binary numbers. -/
 def decode_num : list Γ₀₁ → num
 | [] := num.zero
 | l := decode_pos_num l
 
+/-- A decoding function from `list Γ₀₁` to ℕ. -/
 def decode_nat : list Γ₀₁ → nat := λ l, decode_num l
 
-def encode_pos_num_nonempty (n : pos_num) : (encode_pos_num n) ≠ [] :=
+lemma encode_pos_num_nonempty (n : pos_num) : (encode_pos_num n) ≠ [] :=
 pos_num.cases_on n (list.cons_ne_nil _ _) (λ m, list.cons_ne_nil _ _) (λ m, list.cons_ne_nil _ _)
 
-def encodek_pos_num : ∀ n, (decode_pos_num(encode_pos_num n) ) = n := begin
+lemma encodek_pos_num : ∀ n, (decode_pos_num(encode_pos_num n) ) = n := begin
   intros n,
   induction n with m hm m hm; unfold encode_pos_num decode_pos_num,
   { refl },
@@ -94,7 +101,7 @@ def encodek_pos_num : ∀ n, (decode_pos_num(encode_pos_num n) ) = n := begin
   { exact congr_arg pos_num.bit0 hm }
 end
 
-def encodek_num : ∀ n, (decode_num(encode_num n) ) = n := begin
+lemma encodek_num : ∀ n, (decode_num(encode_num n) ) = n := begin
   intros n,
   cases n, {
     trivial,
@@ -109,20 +116,23 @@ def encodek_num : ∀ n, (decode_num(encode_num n) ) = n := begin
   simp only [pos_num.cast_to_num],
 end
 
-def encodek_nat : ∀ n, (decode_nat(encode_nat n) ) = n := begin
+lemma encodek_nat : ∀ n, (decode_nat(encode_nat n) ) = n := begin
   intro n,
   conv_rhs {rw ← num.to_of_nat n},
   exact congr_arg coe (encodek_num ↑n),
 end
 
+/-- A binary encoding of ℕ in Γ₀₁. -/
 def encoding_nat_Γ₀₁ : encoding ℕ :=
 { Γ := Γ₀₁,
   encode := encode_nat,
   decode := λ n, some (decode_nat n),
   encodek := λ n, congr_arg _ (encodek_nat n) }
 
+/-- A binary fin_encoding of ℕ in Γ₀₁. -/
 def fin_encoding_nat_Γ₀₁ : fin_encoding ℕ := ⟨ encoding_nat_Γ₀₁, Γ₀₁.fintype ⟩
 
+/-- A binary encoding of ℕ in Γ'. -/
 def encoding_nat_Γ' : encoding ℕ :=
 { Γ := Γ',
   encode := λ x, list.map inclusion_Γ₀₁_Γ' (encode_nat x),
@@ -133,17 +143,21 @@ def encoding_nat_Γ' : encoding ℕ :=
     exact encodek_nat x,
   end }
 
+/-- A binary fin_encoding of ℕ in Γ'. -/
 def fin_encoding_nat_Γ' : fin_encoding ℕ := ⟨ encoding_nat_Γ', Γ'.fintype ⟩
 
+/-- A unary encoding function of ℕ in Γ₀₁. -/
 def unary_encode_nat : nat → list Γ₀₁
 | 0 := []
 | (n+1) := Γ₀₁.bit1 :: (unary_encode_nat n)
 
+/-- A unary decoding function from `list Γ₀₁` to ℕ. -/
 def unary_decode_nat : list Γ₀₁ → nat := list.length
 
-def unary_encodek_nat : ∀ n, unary_decode_nat (unary_encode_nat n) = n :=
+lemma unary_encodek_nat : ∀ n, unary_decode_nat (unary_encode_nat n) = n :=
 λ n, nat.rec rfl (λ (m : ℕ) (hm : unary_decode_nat (unary_encode_nat m) = m), (congr_arg nat.succ hm.symm).symm) n
 
+/-- A unary fin_encoding of ℕ. -/
 def unary_fin_encoding_nat : fin_encoding ℕ :=
 { Γ := Γ₀₁,
   encode := unary_encode_nat,
@@ -151,17 +165,20 @@ def unary_fin_encoding_nat : fin_encoding ℕ :=
   encodek := λ n, congr_arg _ (unary_encodek_nat n),
   Γ_fin := Γ₀₁.fintype}
 
+/-- An encoding function of bool in Γ₀₁. -/
 def encode_bool : bool → list Γ₀₁
 | ff := [Γ₀₁.bit0]
 | tt := [Γ₀₁.bit1]
 
+/-- A decoding function from `list Γ₀₁` to bool. -/
 def decode_bool : list Γ₀₁ → bool
 | [Γ₀₁.bit0] := ff
 | [Γ₀₁.bit1] := tt
 | _ := arbitrary bool
 
-def encodek_bool : ∀ b, (decode_bool(encode_bool b)) = b := λ b, bool.cases_on b rfl rfl
+lemma encodek_bool : ∀ b, (decode_bool(encode_bool b)) = b := λ b, bool.cases_on b rfl rfl
 
+/-- A fin_encoding of bool in Γ₀₁. -/
 def fin_encoding_bool_Γ₀₁ : fin_encoding bool :=
 { Γ := Γ₀₁,
   encode := encode_bool,
@@ -169,4 +186,6 @@ def fin_encoding_bool_Γ₀₁ : fin_encoding bool :=
   encodek := λ x, congr_arg _ (encodek_bool x),
   Γ_fin := Γ₀₁.fintype }
 
-end encoding
+instance inhabited_fin_encoding : inhabited (fin_encoding bool) := ⟨fin_encoding_bool_Γ₀₁⟩
+
+instance inhabited_encoding : inhabited (encoding bool) := ⟨fin_encoding_bool_Γ₀₁.to_encoding⟩
